Extract [Is_present_in] from TranslationCorrectness.

TranslationCorrectness.v
@@ -3,6 +3,8 @@ Import List.ListNotations.
 Open Scope list_scope.
 
 Require Import Rustre.Common.
+Open Scope positive.
+
 Require Import Rustre.Heap.
 Require Import Rustre.Dataflow.
 (* TODO: these should go *)
@@ -11,10 +13,10 @@ Require Import Rustre.Dataflow.IsDefined.Decide.
 
 (* ** Definitions on imperative statements *)
 
-Require Import PArith.
 Require Import Rustre.Minimp.
 Require Import Rustre.Translation.
 Require Import Rustre.Translation.Proper.
+Require Import Rustre.Translation.IsPresent.
 
 
 (* TODO:
@@ -37,79 +39,6 @@ Require Import Rustre.Translation.Proper.
      where a clock is active.
  *)
 
-Lemma exp_eval_tovar_Cbool_dec:
-  forall menv env mems c v,
-    {exp_eval menv env (tovar mems c) (Cbool v)}
-    + {~exp_eval menv env (tovar mems c) (Cbool v)}.
-Proof.
-  Ltac no_match := right; inversion_clear 1; try unfold mfind_mem in *;
-                   match goal with
-                   | H: PM.find _ _ = _ |- _ => rewrite H in *; discriminate
-                   end.
-  intros menv env mems c v.
-  unfold tovar.
-  destruct (PS.mem c mems).
-  - case_eq (mfind_mem c menv).
-    + intro c0; destruct c0.
-      * no_match.
-      * destruct b; destruct v; (left; apply estate; assumption) || no_match.
-    + no_match.
-  - case_eq (PM.find c env).
-    + intro c0; destruct c0.
-      * no_match.
-      * destruct b; destruct v; (left; apply evar; assumption) || no_match.
-    + no_match.
-Qed.
-
-Inductive Is_present_in (mems: PS.t) heap stack
-  : clock -> Prop :=
-| IsCbase: Is_present_in mems heap stack Cbase
-| IsCon:
-    forall ck c v,
-      Is_present_in mems heap stack ck
-      -> exp_eval heap stack (tovar mems c) (Cbool v)
-      -> Is_present_in mems heap stack (Con ck c v).
-
-Lemma Is_present_in_dec:
-  forall mems menv env ck,
-    {Is_present_in mems menv env ck}+{~Is_present_in mems menv env ck}.
-Proof.
-  intros.
-  induction ck.
-  - left; constructor.
-  - destruct IHck.
-    + destruct (exp_eval_tovar_Cbool_dec menv env mems i b); destruct b;
-      (left; constructor; assumption) || right; inversion_clear 1; auto.
-    + right; inversion_clear 1; auto.
-Qed.
-
-Inductive Is_absent_in (mems: PS.t) heap stack: clock -> Prop :=
-| IsAbs1:
-    forall ck c v,
-      Is_absent_in mems heap stack ck
-      -> Is_absent_in mems heap stack (Con ck c v)
-| IsAbs2:
-    forall ck c v1 v2,
-         Is_present_in mems heap stack ck
-      -> exp_eval heap stack (tovar mems c) (Cbool v1)
-      -> v2 <> v1
-      -> Is_absent_in mems heap stack (Con ck c v2).
-
-Lemma Is_absent_in_disj:
-  forall mems menv env ck c v,
-    Is_absent_in mems menv env (Con ck c v)
-    -> (Is_absent_in mems menv env ck
-        \/ (forall v', exp_eval menv env (tovar mems c) (Cbool v')
-                       -> v' <> v)).
-Proof.
-  intros mems menv env ck c v.
-  inversion_clear 1 as [|? ? ? ? Hp Hexp Hneq]; intuition.
-  right; intros v' Hexp'.
-  intro HR; rewrite <-HR in *; clear HR.
-  apply Hneq.
-  pose proof (exp_eval_det _ _ _ _ _ Hexp Hexp') as Heq.
-  injection Heq; intuition.
-Qed.
 
 Lemma exp_eval_tovar:
   forall x v menv env memories,
