Translation/IsPresent.v
@@ -1,0 +1,84 @@
+Require Import Rustre.Common.
+Require Import Rustre.Heap.
+Require Import Rustre.Dataflow.
+Require Import Rustre.Minimp.Syntax.
+Require Import Rustre.Minimp.Semantics.
+Require Import Rustre.Translation.
+
+Inductive Is_present_in (mems: PS.t) heap stack
+  : clock -> Prop :=
+| IsCbase: Is_present_in mems heap stack Cbase
+| IsCon:
+    forall ck c v,
+      Is_present_in mems heap stack ck
+      -> exp_eval heap stack (tovar mems c) (Cbool v)
+      -> Is_present_in mems heap stack (Con ck c v).
+
+Inductive Is_absent_in (mems: PS.t) heap stack: clock -> Prop :=
+| IsAbs1:
+    forall ck c v,
+      Is_absent_in mems heap stack ck
+      -> Is_absent_in mems heap stack (Con ck c v)
+| IsAbs2:
+    forall ck c v1 v2,
+         Is_present_in mems heap stack ck
+      -> exp_eval heap stack (tovar mems c) (Cbool v1)
+      -> v2 <> v1
+      -> Is_absent_in mems heap stack (Con ck c v2).
+
+
+Lemma exp_eval_tovar_Cbool_dec:
+  forall menv env mems c v,
+    {exp_eval menv env (tovar mems c) (Cbool v)}
+    + {~exp_eval menv env (tovar mems c) (Cbool v)}.
+Proof.
+  Ltac no_match := right; inversion_clear 1; try unfold mfind_mem in *;
+                   match goal with
+                   | H: PM.find _ _ = _ |- _ => rewrite H in *; discriminate
+                   end.
+  intros menv env mems c v.
+  unfold tovar.
+  destruct (PS.mem c mems).
+  - case_eq (mfind_mem c menv).
+    + intro c0; destruct c0.
+      * no_match.
+      * destruct b; destruct v; (left; apply estate; assumption) || no_match.
+    + no_match.
+  - case_eq (PM.find c env).
+    + intro c0; destruct c0.
+      * no_match.
+      * destruct b; destruct v; (left; apply evar; assumption) || no_match.
+    + no_match.
+Qed.
+
+
+
+Lemma Is_present_in_dec:
+  forall mems menv env ck,
+    {Is_present_in mems menv env ck}+{~Is_present_in mems menv env ck}.
+Proof.
+  intros.
+  induction ck.
+  - left; constructor.
+  - destruct IHck.
+    + destruct (exp_eval_tovar_Cbool_dec menv env mems i b); destruct b;
+      (left; constructor; assumption) || right; inversion_clear 1; auto.
+    + right; inversion_clear 1; auto.
+Qed.
+
+
+Lemma Is_absent_in_disj:
+  forall mems menv env ck c v,
+    Is_absent_in mems menv env (Con ck c v)
+    -> (Is_absent_in mems menv env ck
+        \/ (forall v', exp_eval menv env (tovar mems c) (Cbool v')
+                       -> v' <> v)).
+Proof.
+  intros mems menv env ck c v.
+  inversion_clear 1 as [|? ? ? ? Hp Hexp Hneq]; intuition.
+  right; intros v' Hexp'.
+  intro HR; rewrite <-HR in *; clear HR.
+  apply Hneq.
+  pose proof (exp_eval_det _ _ _ _ _ Hexp Hexp') as Heq.
+  injection Heq; intuition.
+Qed.
